Update materials to class

src/EncryptionSDK/Materials.dfy
@@ -14,20 +14,90 @@ module Materials {
                                                ciphertext : seq<UInt8>)
 
   // TODO: Add keyring trace
-  datatype EncryptionMaterials = EncryptionMaterials(algorithmSuiteID : AlgorithmSuite.ID,
-                                                     encryptedDataKeys : seq<EncryptedDataKey>, 
-                                                     encryptionContext : EncryptionContext, 
-                                                     plaintextDataKey : Option<seq<UInt8>>,
-                                                     signingKey : Option<seq<UInt8>>) {
-    predicate Valid() {
-      |this.encryptedDataKeys| > 0 ==> this.plaintextDataKey.Some?
+  class EncryptionMaterials {
+    var algorithmSuiteID: AlgorithmSuite.ID
+    var encryptedDataKeys: seq<EncryptedDataKey>
+    var encryptionContext: Option<EncryptionContext>
+    var plaintextDataKey: Option<seq<UInt8>>
+    var signingKey: Option<seq<UInt8>>
+
+    predicate Valid() 
+      reads this
+    {
+      |encryptedDataKeys| > 0 ==> plaintextDataKey.Some?
       // TODO data key length assurance
+    }
+    constructor(algorithmSuiteID: AlgorithmSuite.ID,
+                encryptedDataKeys: seq<EncryptedDataKey>, 
+                encryptionContext: Option<EncryptionContext>, 
+                plaintextDataKey: Option<seq<UInt8>>,
+                signingKey: Option<seq<UInt8>>)
+      requires |encryptedDataKeys| > 0 ==> plaintextDataKey.Some?
+      ensures Valid()
+    {
+      this.algorithmSuiteID := algorithmSuiteID;
+      this.encryptedDataKeys := encryptedDataKeys;
+      this.encryptionContext := encryptionContext;
+      this.plaintextDataKey := plaintextDataKey;
+      this.signingKey := signingKey;
+    }
+
+    method setPlaintextDataKey(dataKey: seq<UInt8>)
+      requires Valid()
+      modifies this
+      ensures Valid()
+      ensures algorithmSuiteID == old(algorithmSuiteID)
+      ensures encryptedDataKeys == old(encryptedDataKeys)
+      ensures encryptionContext == old(encryptionContext)
+      ensures signingKey == old(signingKey)
+      ensures plaintextDataKey == Some(dataKey)
+    {
+      plaintextDataKey := Some(dataKey);
+    }
+
+    method appendEncryptedDataKeys(edk: EncryptedDataKey)
+      requires Valid()
+      requires plaintextDataKey.Some?
+      modifies this
+      ensures Valid()
+      ensures plaintextDataKey == old(plaintextDataKey)
+      ensures algorithmSuiteID == old(algorithmSuiteID)
+      ensures encryptionContext == old(encryptionContext)
+      ensures signingKey == old(signingKey)
+      ensures |encryptedDataKeys| > 0
+      ensures encryptedDataKeys[..|encryptedDataKeys|-1] == old(encryptedDataKeys)
+    {
+      encryptedDataKeys := encryptedDataKeys + [edk];
     }
   }
 
   // TODO: Add keyring trace
-  datatype DecryptionMaterials = DecryptionMaterials(algorithmID : AlgorithmSuite.ID,
-                                                     encryptionContext : EncryptionContext,
-                                                     plaintextDataKey : Option<seq<UInt8>>,
-                                                     verificationKey : Option<seq<UInt8>>)
+  class DecryptionMaterials {
+    var algorithmSuiteID: AlgorithmSuite.ID
+    var encryptionContext: Option<EncryptionContext>
+    var plaintextDataKey: Option<seq<UInt8>>
+    var verificationKey: Option<seq<UInt8>>
+    
+    // TODO add Valid()
+
+    constructor(algorithmSuiteID: AlgorithmSuite.ID,
+                encryptionContext: Option<EncryptionContext>,
+                plaintextDataKey: Option<seq<UInt8>>,
+                verificationKey: Option<seq<UInt8>>) {
+      this.algorithmSuiteID := algorithmSuiteID;
+      this.encryptionContext := encryptionContext;
+      this.plaintextDataKey := plaintextDataKey;
+      this.verificationKey := verificationKey;
+    }
+
+    method setPlaintextDataKey(dataKey: seq<UInt8>)
+      modifies this
+      ensures plaintextDataKey == Some(dataKey)
+      ensures algorithmSuiteID == old(algorithmSuiteID)
+      ensures encryptionContext == old(encryptionContext)
+      ensures verificationKey == old(verificationKey)
+    {
+      plaintextDataKey := Some(dataKey);
+    }
+  }
 }
