src/EncryptionSDK/Keyring/Defs.dfy
@@ -4,30 +4,35 @@ include "../Materials.dfy"
 
 module KeyringDefs {
   import opened StandardLibrary
-  import opened UInt = StandardLibrary.UInt
   import opened Materials
 
   trait {:termination false} Keyring {
     ghost var Repr : set<object>
     predicate Valid() reads this, Repr
 
-    method OnEncrypt(x: EncryptionMaterials) returns (res: Result<EncryptionMaterials>)
-      requires x.Valid()
+    method OnEncrypt(encMat: EncryptionMaterials) returns (res: Result<EncryptionMaterials>)
       requires Valid()
+      requires encMat.Valid()
+      modifies encMat
       ensures Valid()
-      ensures res.Ok? ==> res.get.Valid()
-      ensures res.Ok? && x.plaintextDataKey.Some? ==> res.get.plaintextDataKey == x.plaintextDataKey
-      ensures res.Ok? ==> res.get.algorithmSuiteID == x.algorithmSuiteID
-      ensures res.Ok? ==> res.get.encryptionContext == x.encryptionContext
+      ensures res.Success? ==> res.value.Valid()
+      ensures res.Success? && old(encMat.plaintextDataKey.Some?) ==> res.value.plaintextDataKey == old(encMat.plaintextDataKey)
+      ensures res.Success? ==> res.value.algorithmSuiteID == old(encMat.algorithmSuiteID)
+      ensures res.Success? ==> res.value.encryptionContext == old(encMat.encryptionContext)
+      ensures res.Success? ==> res.value.signingKey == old(encMat.signingKey)
       // TODO: keyring trace GENERATED_DATA_KEY flag assurance
       // TODO: keyring trace ENCRYPTED_DATA_KEY flag assurance
 
-    method OnDecrypt(x: DecryptionMaterials, encryptedDataKeys: seq<EncryptedDataKey>) returns (res: Result<DecryptionMaterials>)
-      // TODO: Valid input DecMaterials
+    method OnDecrypt(decMat: DecryptionMaterials, edks: seq<EncryptedDataKey>) returns (res: Result<DecryptionMaterials>)
       requires Valid()
+      // TODO: Valid input DecMaterials
+      modifies decMat
       ensures Valid()
       // TODO: Valid output DecMaterials
-      ensures x.plaintextDataKey.Some? ==> res.Ok? && res.get == x
+      ensures decMat.plaintextDataKey.Some? ==> res.Success? && res.value == decMat
+      ensures res.Success? ==> res.value.algorithmSuiteID == old(decMat.algorithmSuiteID)
+      ensures res.Success? ==> res.value.encryptionContext == old(decMat.encryptionContext)
+      ensures res.Success? ==> res.value.verificationKey == old(decMat.verificationKey)
       // TODO: keyring trace DECRYPTED_DATA_KEY flag assurance
   }
 }
