src/StandardLibrary/StandardLibrary.dfy
@@ -1,5 +1,7 @@
+include "UInt.dfy"
+
 module {:extern "STL"} StandardLibrary {
   datatype Option<T> = None | Some(get: T)
 
-  datatype Result<T> = Ok(get : T) | Err(err : string)
+  datatype Result<T> = Success(value : T) | Failure(error : string)
 }
